\documentclass{article}

\usepackage[utf8]{inputenc}
\usepackage[margin=2cm]{geometry}
\usepackage{amsmath, amsfonts, amssymb, amsthm, mathtools}
\usepackage{graphicx}
\usepackage{parskip}

\title{Title}
\author{Ulrik Bernhardt Danielsen}

\theoremstyle{plain}
\newtheorem{theorem}{Theorem}[section]

\theoremstyle{definition}
\newtheorem{definition}{Definition}[section]

\begin{document}

\maketitle

Assume that the model assumptions for the Cox proportional hazards model holds for a continuous survival time $T$ with covariates $\textbf{Z} = (Z_1, \hdots, Z_p)'$, i.e., that,
\begin{equation*}
        \lambda(t; \textbf{z}) = \lambda_0(t) \exp (\boldsymbol{\beta'z}), 
\end{equation*}
but that the survival times are grouped in the intervals $[0 = a_0, a_1), \hdots, [a_{g-1}, a_g)$.
The corresponding hazards are defined as 
\begin{equation*}
        \lambda_j(\textbf{z}) = P(T < a_j |T \geq a_{j-1}; \textbf{z}), \ j = 1, \hdots, g.
\end{equation*}
Then we can write 
\begin{align*}
        1 - \lambda_j(\textbf{z}) &= P(T \geq a_j | T \geq a_{j-1}; \textbf{z}) \\
                                  &= \frac{P(T \geq a_j, T \geq a_{j-1} ; \textbf{z})}{P(T \geq a_{j-1}; \textbf{z})} \\
                                  &= \frac{P(T \geq a_j; \textbf{z})}{P(T \geq a_{j-1}; \textbf{z})}.
\end{align*}
First we observe that 
\begin{align*}
        P(T \geq a_j ; \textbf{z}) &= S_\textbf{z}(a_j) \\\
                                   &= \exp (- \Lambda_\textbf{z}(a_j)) \\
                                   &= \exp (-(\int_{a_0}^{a_1}\lambda_0(t)\exp (\boldsymbol{\beta'z}dt + \hdots + \int_{a_{j-1}}^{a_j}\lambda_0(t)\exp(\boldsymbol{\beta'z}dt)))) \\
                                   &= \exp (-(\int_{a_0}^{a_1}\lambda_0(t)dt + \hdots + \int_{a_{j-1}}^{a_j}\lambda_0(t)dt)\exp (\boldsymbol{\beta'z})) \\
                                   &= \left( \exp(-\Lambda_\textbf{0}(a_j)) \right)^{\exp (\boldsymbol{\beta'z})} \\
                                   &= (P(T \geq a_j ; \textbf{0}))^{\exp (\boldsymbol{\beta'z})}.
\end{align*}
The exact same argument for $P(T \geq a_{j-1} ; \textbf{z})$ gives us 
\begin{align*}
        1 - \lambda_j(\textbf{z}) &= \left( \frac{P(T \geq a_j; \textbf{0})}{P(T \geq a_{j-1}; \textbf{0})} \right)^{\exp (\boldsymbol{\beta'z})} \\
                                  &= (1 - \lambda_j(\textbf{0}))^{\exp (\boldsymbol{\beta'z})}
\end{align*}
or equivalently
\begin{equation*}
        \log (1 - \lambda_j(\textbf{z})) = (1 - \lambda_j) \exp (\boldsymbol{\beta'z}).
\end{equation*}




\end{document}

